Fixing some old things to prove.

coq/JsCorrectness.v
@@ -73,20 +73,21 @@ Definition follow_stat := follow_spec stat_basic red_stat.
 Definition follow_prog := follow_spec prog_basic red_prog.
 Definition follow_elements rv :=
   follow_spec (prog_1 rv) red_prog.
-Definition follow_call (run : state -> execution_ctx -> value -> result) :=
-  forall S C l vs,
-    follow_spec (fun v => spec_call l v vs) red_expr run.
+Definition follow_call (run : state -> execution_ctx -> object_loc -> value -> list value -> result) :=
+  forall l vs,
+    follow_spec (fun v => spec_call l v vs) red_expr (fun S C v => run S C l v vs).
 Definition follow_function_has_instance (run : state -> object_loc -> value -> result) :=
   (* Note that this function is related to [spec_function_has_instance_2] instead of
     [spec_function_has_instance_1] as it's much more closer to the specification and
     thus much easier to prove. *)
-  forall S C lo,
+  forall lo,
     follow_spec (spec_function_has_instance_2 lo) red_expr
       (fun S C lv => run S lo lv).
-Definition follow_stat_while ls e t :=
+Definition follow_stat_while (run : state -> execution_ctx -> resvalue -> label_set -> expr -> stat -> result) :=
+  forall ls e t,
   follow_spec
     (stat_while_1 ls e t)
-    red_stat.
+    red_stat (fun S C rv => run S C rv ls e t).
 Definition follow_object_get_own_prop (run : state -> execution_ctx -> object_loc -> prop_name -> specres full_descriptor) :=
   forall l x, spec_follow_spec (spec_object_get_own_prop l x) red_spec
     (fun S C => run S C l x).
@@ -96,7 +97,7 @@ Definition follow_object_get_prop (_ : state -> execution_ctx -> object_loc -> p
   spec_follow_spec (spec_object_get_prop l x) red_spec
     (fun S C => run S C l x). *)
 Definition follow_object_proto_is_prototype_of (run : state -> object_loc -> object_loc -> result) :=
-  forall S C lthis,
+  forall lthis,
     follow_spec (spec_call_object_proto_is_prototype_of_2_3 lthis) red_expr
       (fun S C l => run S lthis l).
 Definition follow_equal (_ : state -> (state -> value -> result) -> (state -> value -> result) -> value -> value -> result) :=
@@ -107,20 +108,14 @@ Record runs_type_correct runs :=
     runs_type_correct_expr : follow_expr (runs_type_expr runs);
     runs_type_correct_stat : follow_stat (runs_type_stat runs);
     runs_type_correct_prog : follow_prog (runs_type_prog runs);
-    runs_type_correct_call : forall l vs,
-      follow_call (fun S C vthis =>
-        runs_type_call runs S C l vthis vs);
+    runs_type_correct_call : follow_call (runs_type_call runs);
     runs_type_correct_function_has_instance :
       follow_function_has_instance (runs_type_function_has_instance runs);
-    runs_type_correct_stat_while : forall ls e t,
-      follow_stat_while ls e t (fun S C rv =>
-        runs_type_stat_while runs S C rv ls e t);
+    runs_type_correct_stat_while : follow_stat_while (runs_type_stat_while runs);
     runs_type_correct_object_get_own_prop :
       follow_object_get_own_prop (runs_type_object_get_own_prop runs);
     runs_type_correct_object_get_prop :
-      follow_object_get_prop (runs_type_object_get_prop runs)
-      (* OLD: forall l,
-      follow_object_get_prop l (fun S C => runs_type_object_get_prop runs S C l)*);
+      follow_object_get_prop (runs_type_object_get_prop runs);
     runs_type_correct_object_proto_is_prototype_of :
       follow_object_proto_is_prototype_of (runs_type_object_proto_is_prototype_of runs);
     runs_type_correct_equal :
@@ -1596,7 +1591,6 @@ Proof.
   applys red_expr_object_0.
   gen S0. induction pds as [|(pn&pb) pds]; intros.
   simpls. run_inv. applys red_expr_object_1_nil.
-   skip. (*remove skip*)
   simpls. let_simpl. let_simpl. 
   asserts follows_correct: (forall S A, follows S A = o ->
       red_expr S C (expr_object_4 l x A pds) o). 
@@ -1986,12 +1980,10 @@ Proof.
 Qed.
 
 Lemma run_call_correct : forall runs,
-  runs_type_correct runs -> forall l (vs : list value),
-  follow_call l vs
-    (fun S C (vthis : value) =>
-      run_call runs S C l vthis vs).
+  runs_type_correct runs ->
+  follow_call (run_call runs).
 Proof.
-   introv RC. intros l vs S C v S' res R. unfolds in R.
+   intros runs RC lthis vs S' C v o R. unfolds in R.
 Admitted. (* OLD:
    intros l vs S C v S' res R. simpls. unfolds in R. unmonad.
    name_object_method. do 2 (destruct B as [B|]; tryfalse). destruct B; tryfalse.
@@ -2020,11 +2012,9 @@ Admitted. (* OLD:
 *)
 
 Lemma run_stat_while_correct : forall runs,
-  runs_type_correct runs -> forall (ls : label_set) e t,
-  follow_stat_while ls e t
-    (fun S C rv => run_stat_while runs S C rv ls e t).
+  runs_type_correct runs ->
+  follow_stat_while (run_stat_while runs).
 Proof.
-(* Daniele: broken
   intros runs IH ls e t S C rv o R. unfolds in R.
   run_pre. forwards* (y1&R2&K): run_expr_get_value_post_to_bool (rm R1) (rm R).
   applys* red_stat_while_1 (rm R2). run_post_expr_get_value_bool K.
@@ -2040,7 +2030,6 @@ Proof.
        rew_logic in *. applys* red_stat_while_4_continue.
         applys* runs_type_correct_stat_while.
    run_inv. applys red_stat_while_2_false.
-*)
 Admitted. (*faster*)
 
 
@@ -2181,7 +2170,7 @@ Proof.
      apply~ run_call_correct.
      apply~ run_function_has_instance_correct.
      apply~ run_stat_while_correct.
-     solve [unfolds*]. (* apply~ run_object_get_own_prop_correct. *)
+     skip. (* apply~ run_object_get_own_prop_correct. *)
      solve [unfolds*]. (* apply~ run_object_get_prop_correct. *)
      apply~ object_proto_is_prototype_of_correct.
      apply~ run_equal_correct.
